Add compiler flag for `mk_delay` optimisation

compiler/backend/passes/pure_to_thunkScript.sml
@@ -24,10 +24,12 @@ Definition get_var_name_def:
 End
 
 Definition mk_delay_def:
-  mk_delay (x:thunk_cexp$cexp) =
-    case x of
-    | Force (Var n) => Var n
-    | _             => Delay x
+  mk_delay flag (x:thunk_cexp$cexp) =
+    if flag then
+      case x of
+      | Force (Var n) => Var n
+      | _             => Delay x
+    else Delay x
 End
 
 Definition must_delay_def:
@@ -42,58 +44,58 @@ Definition must_delay_def:
 End
 
 Definition to_thunk_def:
-  to_thunk (s:vars) (pure_cexp$Var c v) =
+  to_thunk flag (s:vars) (pure_cexp$Var c v) =
     (thunk_cexp$Force (Var v),s) ∧
-  to_thunk s (Lam c ns x) =
-    (let (x,s) = to_thunk s x in (Lam ns x,s)) ∧
-  to_thunk s (App c x ys) =
-    (let (x,s) = to_thunk s x in
-     let (ys,s) = to_thunk_list s ys in
-       (App x (MAP mk_delay ys), s)) ∧
-  to_thunk s (Letrec c xs y) =
-    (let (y,s) = to_thunk s y in
-     let (ys,s) = to_thunk_list s (MAP SND xs) in
+  to_thunk flag s (Lam c ns x) =
+    (let (x,s) = to_thunk flag s x in (Lam ns x,s)) ∧
+  to_thunk flag s (App c x ys) =
+    (let (x,s) = to_thunk flag s x in
+     let (ys,s) = to_thunk_list flag s ys in
+       (App x (MAP (mk_delay flag) ys), s)) ∧
+  to_thunk flag s (Letrec c xs y) =
+    (let (y,s) = to_thunk flag s y in
+     let (ys,s) = to_thunk_list flag s (MAP SND xs) in
        (Letrec (MAP2 (λ(n,_) y. (n, Delay y)) xs ys) y,s)) ∧
-  to_thunk s (Let c v x y) =
-    (let (x,s) = to_thunk s x in
-     let (y,s) = to_thunk s y in
-       (Let (SOME v) (mk_delay x) y,s)) ∧
-  to_thunk s (Prim c p ys) =
-    (let (xs,s) = to_thunk_list s ys in
+  to_thunk flag s (Let c v x y) =
+    (let (x,s) = to_thunk flag s x in
+     let (y,s) = to_thunk flag s y in
+       (Let (SOME v) (mk_delay flag x) y,s)) ∧
+  to_thunk flag s (Prim c p ys) =
+    (let (xs,s) = to_thunk_list flag s ys in
        case p of
        | Cons t => (Prim (Cons t) (if must_delay t
                                    then MAP Delay xs
-                                   else MAP mk_delay xs),s)
+                                   else MAP (mk_delay flag) xs),s)
        | AtomOp a => (Prim (AtomOp a) xs,s)
        | Seq =>
            let x = any_el 0 xs in
            let y = any_el 1 xs in
            let (fresh,s) = invent_var (get_var_name ys) s in
              (Let (SOME fresh) x y,s)) ∧
-  to_thunk s (Case c x v ys opt) =
-    (let (x,s) = to_thunk s x in
-     let (rs,s) = to_thunk_list s (MAP (SND o SND) ys) in
+  to_thunk flag s (Case c x v ys opt) =
+    (let (x,s) = to_thunk flag s x in
+     let (rs,s) = to_thunk_list flag s (MAP (SND o SND) ys) in
      let (w,s) = invent_var (v ^ strlit "_forced") s in
        case opt of
        | NONE =>
-           ((Let (SOME v) (mk_delay x) $
+           ((Let (SOME v) (mk_delay flag x) $
              Let (SOME w) (Force (Var v)) $
               Case w (MAP2 (λ(c,n,_) y. (c,n,y)) ys rs) NONE,s))
        | SOME (a,y) =>
-          let (y,s) = to_thunk s y in
-            ((Let (SOME v) (mk_delay x) $
+          let (y,s) = to_thunk flag s y in
+            ((Let (SOME v) (mk_delay flag x) $
               Let (SOME w) (Force (Var v)) $
                Case w (MAP2 (λ(c,n,_) y. (c,n,y)) ys rs) (SOME (a,y))),s)) ∧
-  to_thunk s (NestedCase c g gv p e pes) = to_thunk s e ∧
-  to_thunk_list s [] = ([],s) ∧
-  to_thunk_list s (x::xs) =
-    (let (x,s) = to_thunk s x in
-     let (xs,s) = to_thunk_list s xs in
+  to_thunk flag s (NestedCase c g gv p e pes) = to_thunk flag s e ∧
+  to_thunk_list flag s [] = ([],s) ∧
+  to_thunk_list flag s (x::xs) =
+    (let (x,s) = to_thunk flag s x in
+     let (xs,s) = to_thunk_list flag s xs in
        (x::xs,s))
 Termination
   WF_REL_TAC `measure $ λx. case x of
-              | INL x => cexp_size (K 0) (SND x)
-              | INR x => list_size (cexp_size (K 0)) (SND x)`
+              | INL (_,_,e) => cexp_size (K 0) e
+              | INR (_,_,l) => list_size (cexp_size (K 0)) l`
   \\ fs [pure_cexpTheory.cexp_size_eq] \\ rw []
   >~ [‘list_size (cexp_size (K 0)) (MAP SND xs)’] >-
     (pop_assum kall_tac
@@ -106,7 +108,7 @@ End
 
 Definition compile_to_thunk_def:
   compile_to_thunk (c:compiler_opts) e =
-    let (e1, vs) = to_thunk (pure_names e) e in
+    let (e1, vs) = to_thunk c.do_mk_delay (pure_names e) e in
     let (e2, vs2) = split_delated_lam c.do_split_dlam e1 vs in
       e2
 End
