compiler/backend/passes/pure_comp_confScript.sml
@@ -11,7 +11,8 @@ Datatype:
       do_pure_sort  : bool ;  (* pure-to-pure binding group analysis *)
       do_pure_clean : bool ;  (* pure-to-pure cleaning / deadcode elimination *)
       do_demands    : bool ;  (* demand analysis *)
-      do_split_dlam : bool ;  (* thunk-to-thunk *)
+      do_mk_delay   : bool ;  (* thunk-to-thunk smart mk_delay constructor *)
+      do_split_dlam : bool ;  (* thunk-to-thunk split delayed lambdas *)
       do_app_unit   : bool    (* state-to-state *)
     |>
 End
@@ -19,6 +20,7 @@ End
 Overload pure_sort_flag[local]  = “strlit "-sort"”
 Overload pure_clean_flag[local] = “strlit "-clean"”
 Overload demands_flag[local]    = “strlit "-demands"”
+Overload mk_delay_flag[local]   = “strlit "-mk_delay"”
 Overload dlam_flag[local]       = “strlit "-dlam"”
 Overload unit_flag[local]       = “strlit "-unit"”
 
@@ -26,6 +28,7 @@ Definition all_flags_def:
   all_flags = [pure_sort_flag;
                pure_clean_flag;
                demands_flag;
+               mk_delay_flag;
                dlam_flag;
                unit_flag]
 End
@@ -37,7 +40,8 @@ Definition read_cline_args_def:
     | [] => INL <| do_pure_sort  := ¬ MEM pure_sort_flag cl  ;
                    do_pure_clean := ¬ MEM pure_clean_flag cl ;
                    do_demands    := ¬ MEM demands_flag cl    ;
-                   do_split_dlam := ¬ MEM dlam_flag cl       ;
+                   do_mk_delay   := ¬ MEM dlam_flag cl       ;
+                   do_split_dlam := ¬ MEM mk_delay_flag cl   ;
                    do_app_unit   := ¬ MEM unit_flag cl       |>
 End
 
